

Exercice 1 :

1. $A = (-3)^5 \times (-3)^2 =$

6. $F = (-4)^5 \times (-4)^3 =$

2. $B = (-4)^4 \times (-4)^3 =$

7. $G = (-3)^3 \times (-3)^2 =$

3. $C = (-5)^3 \times (-5)^2 =$

8. $H = (-6)^4 \times (-6)^2 =$

4. $D = (-3)^5 \times (-3)^3 =$

9. $I = (-2)^4 \times (-2)^3 =$

5. $E = (-4)^3 \times (-4)^2 =$

10. $J = (-5)^5 \times (-5)^2 =$

Exercice 2 :

1. $A = \frac{(-8)^3}{(-8)^2} =$

6. $F = \frac{(-6)^5}{(-6)^2} =$

2. $B = \frac{(-2)^5}{(-2)^4} =$

7. $G = \frac{(-5)^4}{(-5)^2} =$

3. $C = \frac{(-3)^4}{(-3)^3} =$

8. $H = \frac{(-4)^3}{(-4)^2} =$

4. $D = \frac{(-8)^5}{(-8)^4} =$

9. $I = \frac{(-3)^3}{(-3)^2} =$

5. $E = \frac{(-7)^4}{(-7)^2} =$

10. $J = \frac{(-6)^4}{(-6)^2} =$

Exercice 3 :

1. $A = (7^4)^2 =$

6. $F = (4^4)^2 =$

2. $B = (7^2)^2 =$

7. $G = ((-2)^4)^3 =$

3. $C = ((-2)^2)^2 =$

8. $H = ((-3)^4)^4 =$

4. $D = ((-2)^3)^3 =$

9. $I = ((-8)^4)^2 =$

5. $E = (8^2)^3 =$

10. $J = (8^3)^3 =$

Exercice 4 :

1. $A = 8^3 \times 5^3 =$

6. $F = 5^3 \times 8^3 =$

2. $B = (-3)^5 \times (-7)^5 =$

7. $G = (-5)^2 \times 3^2 =$

3. $C = 7^3 \times 5^3 =$

8. $H = 2^4 \times 5^4 =$

4. $D = (-7)^5 \times 5^5 =$

9. $I = (-2)^4 \times 8^4 =$

5. $E = 8^3 \times 3^3 =$

10. $J = (-5)^2 \times (-3)^2 =$

Exercice 5 :

1. $A = \frac{15^5}{(-5)^5} =$

6. $F = \frac{(-6)^4}{2^4} =$

2. $B = \frac{(-20)^2}{(-5)^2} =$

7. $G = \frac{6^4}{2^4} =$

3. $C = \frac{(-6)^4}{(-2)^4} =$

8. $H = \frac{(-9)^4}{3^4} =$

4. $D = \frac{(-12)^2}{(-3)^2} =$

9. $I = \frac{(-4)^3}{(-2)^3} =$

5. $E = \frac{(-8)^2}{(-2)^2} =$

10. $J = \frac{8^2}{2^2} =$